recovering original file

examples/security/statefulEnc-multi-frame-orig.fst
@@ -1,8 +1,8 @@
 (*--build-config
-    options:--admit_fsi Set --admit_fsi Seq --z3timeout 15 --max_fuel 1 --max_ifuel 1 --initial_ifuel 1 --max_ifuel 1;
+    options:--admit_fsi Set --admit_fsi Seq --z3timeout 15 --max_fuel 1 --max_ifuel 1 --initial_ifuel 1 --initial_fuel 1;
     other-files:../../lib/ext.fst ../../lib/set.fsi ../../lib/heap.fst ../../lib/st.fst ../../lib/seq.fsi ../../lib/list.fst
   --*)
-(* A standalone experiment corresponding to building stateful encryption on
+(* A standalone experiment corresponding to building a stateful encryption on
    top of a stateless one ... along the lines of StatefulLHAE on top of AEAD_GCM *)
 module StatefulEncryption.MultiInstance.Frame
 open ST
@@ -37,9 +37,6 @@ let rec find_seq' a f s i =
 let find_seq a f s = find_seq' #a f s 0
 *)
 
-assume val seq_map: #a:Type -> #b:Type -> f:(a -> Tot b) -> s:seq a ->
-  Tot (t:seq b { Seq.length t = Seq.length s /\ (forall (i:nat{i < Seq.length s}).(Seq.index t i = f (Seq.index s i))) })
-
 // replacing the usual modifies clause?
 // this does not preclude h' extending h with fresh refs
 opaque logic type modifies (mods:set aref) (h:heap) (h':heap) =
@@ -50,34 +47,29 @@ type Fresh (#a:Type) h0 (r:ref a) h1 = Heap.contains h1 r /\ not (Heap.contains 
 type Let (#a:Type) (x:a) (body: (y:a{y=x} -> Type)) = body x
 
 (* ------------------------------------------------------------ *)
-(* Start with a basic possibly-stateful encryption functionality *)
+(* Start with a basic stateful encryption functionality *)
 
 (* Some placeholder functions to build plain/cipher/key *)
 
 type key
-// we need something possibly stateful, accounting for random sampling & pairwise distinct keys
+// we need something more stateful, accounting for random sampling & pairwise distinct keys
 // similarly we should be able to instantiate the scheme to an instance that holds/updates refs in key
 
-// assume val gen0: unit -> Tot key
-assume val gen0: unit -> St key (fun h -> True) (fun h0 k h1 -> modifies !{} h0 h1)
+// assume val mk_key: unit -> Tot key
+assume val mk_key: unit -> ST key (fun h -> True) (fun h0 k h1 -> modifies !{} h0 h1)
 
 type plain
-assume val mk_plain: unit -> St plain (fun h -> True) (fun h0 k h1 -> modifies !{} h0 h1)
-
-type ad = nat // additional data, just integers for simplicity
+assume val mk_plain: unit -> ST plain (fun h -> True) (fun h0 k h1 -> modifies !{} h0 h1)
 
 type cipher
-assume val enc0: s:seq cipher (* ghost *) -> St cipher
-  (fun h -> True)
-  (fun h0 c h1 -> modifies !{} h0 h1
-               /\ find_seq (fun c' -> c=c') s = None)
+assume val mk_cipher: unit -> ST cipher (fun h -> True) (fun h0 k h1 -> modifies !{} h0 h1)
 
 // to guarantees that decryption is a stateful inverse of encryption (a good sanity check),
 // the invariant on entries should state that the ciphers are pairwise distinct.
 // we may also have a refinement guaranteeing that decryption of that ciphertext yields that plaintext.
 
 type basicEntry =
-  | Entry : i:ad -> c:cipher -> p:plain -> basicEntry
+  | Entry : p:plain -> c:cipher -> basicEntry
 
 type encryptor =
   | Enc : log:ref (seq basicEntry) -> key -> encryptor
@@ -90,6 +82,7 @@ type paired (e:encryptor) (d:decryptor) = b2t (Enc.log e = Dec.log d)
 (* A basic instance *)
 type bi =
   | BI : e:encryptor -> d:decryptor{paired e d} -> bi
+opaque logic type triggerBI (x:bi) = True
 
 // new concrete syntax for sets of (a & x:a) ?
 let bi_refs (BI e d) = !{Enc.log e}
@@ -103,20 +96,22 @@ type pairwise_distinct (s:list bi) =
 (* basic_fp: the footprint of the basic encryption functionality.
              maintains all basic instances, bi
 *)
-let basic_fp : ref (s:list bi{pairwise_distinct s}) = ref []
+let basic_fp : ref (list bi) = ref []
 
 // somewhat generic
 // could we put the separation from basic_fp above instead?
 // could we show that those refs are separated from others?
 type basic_fp_inv (h:heap) =
   Heap.contains h basic_fp
-  /\ (forall bi.
-        List.mem bi (Heap.sel h basic_fp)
-         ==> (forall (a:Type) (r:ref a).
-                Set.mem (Ref r) (bi_refs bi)
-                ==> Heap.contains h r /\ r =!= basic_fp))
+  /\ (forall bi.{:pattern (triggerBI bi)}
+        triggerBI bi
+        /\ List.mem bi (Heap.sel h basic_fp)
+         ==> (forall bi'.{:pattern (triggerBI bi')} triggerBI bi' /\ List.mem bi' (Heap.sel h basic_fp) ==> bi=bi' \/ distinct_bi bi bi')
+             /\ (forall (a:Type) (r:ref a).
+                    Set.mem (Ref r) (bi_refs bi)
+                    ==> Heap.contains h r /\ r =!= basic_fp))
 
-val gen: unit -> St bi
+val gen: unit -> ST bi
   (requires (basic_fp_inv))
   (ensures (fun h0 b h1 ->
       modifies !{basic_fp} h0 h1
@@ -126,7 +121,7 @@ val gen: unit -> St bi
          Fresh h0 log h1
          /\ Heap.sel h1 log = emp)))
 let gen () =
-  let key = gen0 () in
+  let key = mk_key () in
   let log = ref emp in
   let bi = BI (Enc log key) (Dec log key) in
   basic_fp := bi::!basic_fp; //ghost
@@ -136,75 +131,75 @@ type in_basic_fp bi h =
   basic_fp_inv h /\
   b2t(List.mem bi (Heap.sel h basic_fp))
 
-type enc_in_basic_fp (e:encryptor) (h:heap) = exists d. paired e d /\ in_basic_fp (BI e d) h
-type dec_in_basic_fp (d:decryptor) (h:heap) = exists e. paired e d /\ in_basic_fp (BI e d) h
+ type enc_in_basic_fp (e:encryptor) (h:heap) = exists d. paired e d /\ in_basic_fp (BI e d) h /\ triggerBI (BI e d)
+ type dec_in_basic_fp (d:decryptor) (h:heap) = exists e. paired e d /\ in_basic_fp (BI e d) h /\ triggerBI (BI e d)
 
-val enc : e:encryptor -> i:ad -> p:plain -> St cipher
-    (requires (fun h -> enc_in_basic_fp e h))
+val enc : e:encryptor -> p:plain -> ST cipher
+    (requires (fun h -> enc_in_basic_fp e h /\ basic_fp_inv h))
     (ensures (fun h0 c h1 ->
                 modifies !{Enc.log e} h0 h1
                 /\ enc_in_basic_fp e h1
-                // /\ Heap.contains h1 (Enc.log e) // could we get it from the precondition?
-                /\ Heap.sel h1 (Enc.log e) = snoc (Heap.sel h0 (Enc.log e)) (Entry i c p)))
-let enc e i p =
-  // failing: let s = seq_map #basicEntry #cipher (fun (e:basicEntry) -> Entry.c e) !(Enc.log e) in
-  let c = enc0 emp in
-  Enc.log e := snoc !(Enc.log e) (Entry i c p);
+                /\ basic_fp_inv h1
+                /\ Heap.sel h1 (Enc.log e) = snoc (Heap.sel h0 (Enc.log e)) (Entry p c)))
+let enc e p =
+  let c = mk_cipher () in
+  Enc.log e := snoc !(Enc.log e) (Entry p c);
   c
 
-let basicMatch i c (Entry i' c' p) = i = i' && c = c'
-
 // cryptographically, this assumes both INT-CTXT and IND-CPA (except for distinct ciphers)
-val dec: d:decryptor -> a:ad -> c:cipher -> St (option plain)
-  (requires (fun h -> dec_in_basic_fp d h))
-  (ensures (fun h0 o h1 ->
+val dec: d:decryptor -> c:cipher -> ST (option plain)
+  (requires (fun h -> dec_in_basic_fp d h /\ basic_fp_inv h))
+  (ensures (fun h0 p h1 ->
               modifies !{} h0 h1
               /\ dec_in_basic_fp d h1
+              /\ basic_fp_inv h1
               /\ (Let (Heap.sel h0 (Dec.log d))
                       (fun log ->
-                          (is_None o <==> (forall (i:nat{i < Seq.length log}).{:pattern (trigger i)} trigger i /\ ~(basicMatch a c (Seq.index log i))))
-                          /\ (is_Some o ==> (exists (i:nat{i < Seq.length log}).{:pattern (trigger i)} trigger i /\ basicMatch a c (Seq.index log i) /\ Entry.p (Seq.index log i) = Some.v o))))))
-let dec d a c =
+                          (is_None p <==> (forall (i:nat{i < Seq.length log}).{:pattern (trigger i)} trigger i /\ Entry.c (Seq.index log i) <> c))
+                          /\ (is_Some p ==> (exists (i:nat{i < Seq.length log}).{:pattern (trigger i)} trigger i /\ Seq.index log i = Entry (Some.v p) c))))))
+let dec d c =
   let s = !(Dec.log d) in
-  match find_seq (basicMatch a c) s with
+  match find_seq (function Entry p c' -> c=c') s with
     | None -> None
     | Some i ->
       cut (trigger i);
       Some (Entry.p (Seq.index s i))
 
-val test_basic_frame : b1:bi -> b2:bi{distinct_bi b1 b2} -> St unit
+
+val test_basic_frame : b1:bi -> b2:bi{distinct_bi b1 b2} -> ST unit
     (requires (fun h ->
-                       in_basic_fp b1 h
+                       basic_fp_inv h
+                    /\ in_basic_fp b1 h
                     /\ in_basic_fp b2 h
                     /\ Heap.sel h (Enc.log (BI.e b1)) = emp
                     /\ Heap.sel h (Enc.log (BI.e b2)) = emp))
     (ensures (fun h0 _ h1 ->
                 basic_fp_inv h1
-                /\ modifies (Set.union (bi_refs b1) (bi_refs b2)) h0 h1))
+                /\ modifies (Set.union !{basic_fp}
+                                        (Set.union (bi_refs b1) (bi_refs b2)))
+                                h0 h1))
 (* A test of multiple basic instances:
      proves that use of one instance doesn't mess with another
 *)
 let test_basic_frame b1 b2 =
-  // let b3 = gen() in // this breaks typing; why?
+  let b3 = gen() in
   let p = mk_plain () in
   let q = mk_plain () in
-  let c0 = enc (BI.e b1) 0 p in
-  let c1 = enc (BI.e b1) 1 q in
-  let c2 = enc (BI.e b2) 0 q in
-  let o0 = dec (BI.d b1) 0 c0 in
-  let o2 = dec (BI.d b2) 0 c2 in
-  let oX = dec (BI.d b1) 2 c0 in // this fails with 1, as we might have c0=c1
-  cut (trigger 0); // what does this achieve?
-  assert (Some.v o0 = p);
-  assert (Some.v o2 = q);
-  assert (oX = None)
+  let c1 = enc (BI.e b1) p in
+  //  let c1'= enc (BI.e b1) q in // this (correctly) breaks typing, unless we strengthen our invariant
+  let c2 = enc (BI.e b2) q in
+  let p' = dec (BI.d b1) c1 in
+  let q' = dec (BI.d b2) c2 in
+  cut (trigger 0);
+  assert (Some.v p' = p);
+  assert (Some.v q' = q)
 
 (* -------------------------------------------------------- *)
 (* This is the analog of StatefulLHAE on top of AEAD_GCM *)
 type statefulEntry =
-  | StEntry : c:cipher -> p:plain -> statefulEntry
+  | StEntry : i:nat -> p:plain -> c:cipher -> statefulEntry
 
-// we used to have a copy of i inside each entry; now gone
+// it is a bit strange to have a copy of the sequence index
 // as above, we could use a stronger invariant
 
 type st_encryptor =
@@ -226,8 +221,12 @@ type st_paired (enc:st_encryptor) (dec:st_decryptor) =
 (* a stateful instance *)
 type sti =
   | STI : e:st_encryptor -> d:st_decryptor{st_paired e d} -> sti
+opaque logic type triggerSTI (x:sti) = True
 
+(* an abstract function to add additional data to the plain text *)
+assume val with_seqn : nat -> plain -> Tot plain
 // this is simplified from AEAD (usually not encrypted)
+// we will need it to be injective in its first argument
 
 (* The invariant of a single instance *)
 type st_inv (e:st_encryptor) (d:st_decryptor) (h:heap) =
@@ -245,13 +244,8 @@ type st_inv (e:st_encryptor) (d:st_decryptor) (h:heap) =
       /\ r <= w              //read counter is before it
       /\ (forall (i:nat{i < Seq.length st}).
           Let (Seq.index st i) (fun st_en ->
-            b2t (Seq.index basic i = Entry i (StEntry.c st_en) (StEntry.p st_en) )))))))
-
-type st_enc_inv (e:st_encryptor) (h:heap) =
-  exists (d:st_decryptor). st_paired e d /\ st_inv e d h
-
-type st_dec_inv (d:st_decryptor) (h:heap) =
-  exists (e:st_encryptor). st_paired e d /\ st_inv e d h
+            StEntry.i st_en = i  //the log is in sync with the basic log, with the ith entry containing i as the additional data
+            /\ Seq.index basic i = Entry (with_seqn i (StEntry.p st_en)) (StEntry.c st_en)))))))
 
 let sti_refs (STI e d) =
   Set.union !{StEnc.log e, StEnc.ctr e, StDec.ctr d}
@@ -266,9 +260,12 @@ type st_fp_inv (h:heap) =
    basic_fp_inv h              //the basic encryption invariant
    /\ Heap.contains h st_fp
    /\ basic_fp =!= st_fp       //two footprints are anti-aliased
-   /\ (forall s1.
-          List.mem s1 (Heap.sel h st_fp)
-          ==> (forall s2. List.mem s2 (Heap.sel h st_fp) ==> s1 = s2 \/ distinct_sti s1 s2) //pairwise distinct
+   /\ (forall s1.{:pattern (triggerSTI s1)}
+          triggerSTI s1
+          /\ List.mem s1 (Heap.sel h st_fp)
+          ==> (forall s2.{:pattern (triggerSTI s2)}
+                    triggerSTI s2
+                    /\ List.mem s2 (Heap.sel h st_fp) ==> s1 = s2 \/ distinct_sti s1 s2) //pairwise distinct
                /\ in_basic_fp (BI (StEnc.key (STI.e s1)) (StDec.key (STI.d s1))) h //the key is in the basic invariant
                /\ st_inv (STI.e s1) (STI.d s1) h //and in the st invariant
                /\ (forall (a:Type) (r:ref a).
@@ -280,7 +277,7 @@ type st_fp_inv (h:heap) =
 let refs_in_e (e:st_encryptor) = !{StEnc.log e, StEnc.ctr e, Enc.log (StEnc.key e)}
 let refs_in_d (d:st_decryptor) = !{StDec.log d, StDec.ctr d, Dec.log (StDec.key d)}
 
-val stateful_gen : unit -> St sti
+val stateful_gen : unit -> ST sti
   (requires (st_fp_inv))
   (ensures (fun h0 b h1 ->
               st_fp_inv h1
@@ -297,75 +294,80 @@ let stateful_gen () =
   st_fp := sti :: !st_fp; //ghost
   sti
 
-type in_st_fp sti h =
-  st_fp_inv h /\
-  b2t( List.mem sti (Heap.sel h st_fp))
+let in_st_fp sti h = List.mem sti (Heap.sel h st_fp)
 
-type enc_in_st_fp (e:st_encryptor) (h:heap) = exists d. st_paired e d /\ in_st_fp (STI e d) h
-type dec_in_st_fp (d:st_decryptor) (h:heap) = exists e. st_paired e d /\ in_st_fp (STI e d) h
+type enc_in_st_fp (e:st_encryptor) (h:heap) =
+  exists d. st_paired e d /\ in_st_fp (STI e d) h /\ triggerSTI (STI e d)
 
-val stateful_enc : e:st_encryptor -> p:plain -> St cipher
-  (requires (fun h -> enc_in_st_fp e h))
+type dec_in_st_fp (d:st_decryptor) (h:heap) =
+  exists e. st_paired e d /\ List.mem (STI e d) (Heap.sel h st_fp) /\ triggerSTI (STI e d)
+
+val stateful_enc : e:st_encryptor -> p:plain -> ST cipher
+  (requires (fun h -> st_fp_inv h /\ enc_in_st_fp e h))
   (ensures (fun h0 c h1 ->
-                    enc_in_st_fp e h1
+                 st_fp_inv h1
                  /\ modifies (refs_in_e e) h0 h1
                  /\ Heap.sel h1 (StEnc.log e) //exactly plain added to the end of the log
-                     = snoc (Heap.sel h0 (StEnc.log e)) (StEntry c p)))
-let stateful_enc (StEnc log ctr e) p =
-  let c = enc e !ctr p in
-  log := snoc !log (StEntry c p);
-  ctr := !ctr + 1;
+                    = snoc (Heap.sel h0 (StEnc.log e)) (StEntry (Heap.sel h0 (StEnc.ctr e)) p c)))
+let stateful_enc e p =
+  let i = !(StEnc.ctr e) in
+  let ip = with_seqn i p in
+  let c = enc (StEnc.key e) ip in
+  StEnc.log e := snoc !(StEnc.log e) (StEntry i p c);
+  StEnc.ctr e := i + 1;
   c
 
-val stateful_dec: d:st_decryptor -> c:cipher -> St (option plain)
-  (requires (fun h -> dec_in_st_fp d h))
+
+val stateful_dec: ad:nat -> d:st_decryptor -> c:cipher -> ST (option plain)
+  (requires (fun h -> st_fp_inv h /\ dec_in_st_fp d h))
   (ensures (fun h0 p h1 ->
-                   dec_in_st_fp d h0 //repeating pre
-                /\ dec_in_st_fp d h1
+                st_fp_inv h0
+                /\ dec_in_st_fp d h0 //repeating pre
+                /\ st_fp_inv h1
                 /\ modifies !{StDec.ctr d} h0 h1
                 /\ Let (Heap.sel h0 (StDec.ctr d)) (fun (r:nat{r=Heap.sel h0 (StDec.ctr d)}) ->
                    Let (Heap.sel h0 (StDec.log d)) (fun (log:seq statefulEntry{log=Heap.sel h0 (StDec.log d)}) ->
                     (is_None p ==> (r = Seq.length log                     //nothing encrypted yet
-                                    || StEntry.c (Seq.index log r) <> c    //wrong cipher
-                                    ) /\ Heap.sel h1 (StDec.ctr d) = r)
+                                    || StEntry.c (Seq.index log r) <> c    //bogus cipher
+                                    || r <> ad))                           //reading at the wrong postition
                    /\ (is_Some p ==>
                           ((Heap.sel h1 (StDec.ctr d) = r + 1)
                            /\ StEntry.p (Seq.index log r) = Some.v p))))))
-
-// note that we do not increment the counter in case of decryption failure,
-// thereby enabling retries
-let stateful_dec (StDec _ ctr d) c =
-  let i = !ctr in
-  cut(trigger i); // what does it do?
-  match dec d !ctr c with
-    | None -> None
-    | Some p -> ctr := !ctr + 1; Some p
-
-// what does it do? related to transient failures?
 #reset-options
-val test_st_frame : s1:sti -> s2:sti{distinct_sti s1 s2} -> St unit
-    (requires (fun h ->
-                   in_st_fp s1 h
-                /\ in_st_fp s2 h
-                /\ Heap.sel h (StEnc.ctr (STI.e s1)) = Heap.sel h (StDec.ctr (STI.d s1))
-             // /\ Heap.sel h (StEnc.ctr (STI.e s2)) = Heap.sel h (StDec.ctr (STI.d s2))
-                    ))
-    (ensures (fun h0 _ h1 ->
-                   in_st_fp s1 h1
-                /\ in_st_fp s2 h1
-                /\ modifies (Set.union (sti_refs s1) (sti_refs s2)) h0 h1))
-// note that we do not require new encryptor/decryptors,
-// just that those in s1 are in sync, so that decryption cancels encryption
+let stateful_dec ad d c =
+  let i = !(StDec.ctr d) in
+  cut(trigger i);
+  match dec (StDec.key d) c with
+    | None ->  None
+    | Some p ->
+      let l = !(StDec.log d) in
+      if i < Seq.length l
+      then let StEntry _ q _ = Seq.index l i in
+           if i = ad
+           then (StDec.ctr d := i + 1; Some q)
+           else None
+      else None
 
+#reset-options
+val test_st_frame : s1:sti -> s2:sti{distinct_sti s1 s2} -> ST unit
+    (requires (fun h -> st_fp_inv h
+                    /\ in_st_fp s1 h
+                    /\ in_st_fp s2 h
+                    /\ Heap.sel h (StEnc.ctr (STI.e s1))
+                       = Heap.sel h (StDec.ctr (STI.d s1))
+                    /\ Heap.sel h (StEnc.ctr (STI.e s2))
+                       = Heap.sel h (StDec.ctr (STI.d s2))))
+    (ensures (fun h0 _ h1 ->
+                st_fp_inv h1
+                /\ modifies (Set.union (sti_refs s1) (sti_refs s2)) h0 h1))
 let test_st_frame s1 s2 =
-  let p = mk_plain () in
-  let q = mk_plain () in
-  // let s3 = stateful_gen() // also type-breaking
-  let c0 = stateful_enc (STI.e s1) p in
-  let c1 = stateful_enc (STI.e s1) q in
-  let c2 = stateful_enc (STI.e s2) p in
-  // let oX = stateful_dec (STI.d s1) c2 in // might succeed
-  let o0 = stateful_dec (STI.d s1) c0 in
-  let o1 = stateful_dec (STI.d s1) c1 in
-  assert (Some.v o0 = p);
-  assert (Some.v o1 = q)
+  let p1 = mk_plain () in
+  let p2 = mk_plain () in
+  let c1 = stateful_enc (STI.e s1) p1 in
+  let c2 = stateful_enc (STI.e s2) p2 in
+  let n1 = !(StDec.ctr (STI.d s1)) in
+  let p1' = stateful_dec n1 (STI.d s1) c1 in
+  let n2 = !(StDec.ctr (STI.d s2)) in
+  let p2' = stateful_dec n2 (STI.d s2) c2 in
+  assert (is_Some p1' /\ Some.v p1' = p1);
+  assert (is_Some p2' /\ Some.v p2' = p2)
